Weidenbach_Book/IsaSAT/IsaSAT_Conflict_Analysis_LLVM.thy
@@ -1,49 +1,6 @@
 theory IsaSAT_Conflict_Analysis_LLVM
 imports IsaSAT_Conflict_Analysis IsaSAT_VMTF_LLVM IsaSAT_Setup_LLVM IsaSAT_LBD_LLVM
 begin
-thm fold_tuple_optimizations
-(*
-lemma mark_of_refine[sepref_fr_rules]:
-  \<open>(return o (\<lambda>C. the (snd C)), RETURN o mark_of) \<in>
-    [\<lambda>C. is_proped C]\<^sub>a pair_nat_ann_lit_assn\<^sup>k \<rightarrow> nat_assn\<close>
-  apply sepref_to_hoare
-  apply (case_tac x; case_tac xi; case_tac \<open>snd xi\<close>)
-  by (sep_auto simp: nat_ann_lit_rel_def)+
-
-
-lemma mark_of_fast_refine[sepref_fr_rules]:
-  \<open>(return o (\<lambda>C. the (snd C)), RETURN o mark_of) \<in>
-    [\<lambda>C. is_proped C]\<^sub>a pair_nat_ann_lit_fast_assn\<^sup>k \<rightarrow> uint64_nat_assn\<close>
-proof -
-  have 1: \<open>option_assn (\<lambda>a c. \<up> ((c, a) \<in> uint64_nat_rel)) = pure (\<langle>uint64_nat_rel\<rangle>option_rel)\<close>
-    unfolding option_assn_pure_conv[symmetric]
-    by (auto simp: pure_def)
-  show ?thesis
-    apply sepref_to_hoare
-    unfolding 1
-    apply (case_tac x; case_tac xi; case_tac \<open>snd xi\<close>)
-       apply (sep_auto simp: br_def)
-      apply (sep_auto simp: nat_ann_lit_rel_def uint64_nat_rel_def br_def
-        ann_lit_of_pair_if cong: )+
-     apply (sep_auto simp: hr_comp_def)
-    apply (sep_auto simp: hr_comp_def uint64_nat_rel_def br_def)
-     apply (auto simp: nat_ann_lit_rel_def elim: option_relE)[]
-    apply (auto simp: ent_refl_true)
-    done
-qed
-*)
-
-lemma get_count_max_lvls_heur_def:
-   \<open>get_count_max_lvls_heur = (\<lambda>(_, _, _, _, _, _, clvls, _). clvls)\<close>
-  by (auto intro!: ext)
-
-sepref_def get_count_max_lvls_heur_impl
-  is \<open>RETURN o get_count_max_lvls_heur\<close>
-  :: \<open>isasat_bounded_assn\<^sup>k \<rightarrow>\<^sub>a uint32_nat_assn\<close>
-  unfolding get_count_max_lvls_heur_def isasat_bounded_assn_def
-  by sepref
-
-lemmas [sepref_fr_rules] = get_count_max_lvls_heur_impl.refine
 
 sepref_def maximum_level_removed_eq_count_dec_fast_code
   is \<open>uncurry (maximum_level_removed_eq_count_dec_heur)\<close>
@@ -51,9 +8,6 @@ sepref_def maximum_level_removed_eq_count_dec_fast_code
   unfolding maximum_level_removed_eq_count_dec_heur_def
   apply (annot_unat_const \<open>TYPE(32)\<close>)
   by sepref
-
-declare
-  maximum_level_removed_eq_count_dec_fast_code.refine[sepref_fr_rules]
 
 lemma is_decided_hd_trail_wl_heur_alt_def:
   \<open>is_decided_hd_trail_wl_heur = (\<lambda>((M, xs, lvls, reasons, k), _).
@@ -72,9 +26,6 @@ sepref_def is_decided_hd_trail_wl_fast_code
     last_trail_pol_pre_def
   by sepref
 
-declare
-  is_decided_hd_trail_wl_fast_code.refine[sepref_fr_rules]
-
 sepref_def lit_and_ann_of_propagated_st_heur_fast_code
   is \<open>lit_and_ann_of_propagated_st_heur\<close>
   :: \<open>[\<lambda>_. True]\<^sub>a
@@ -86,34 +37,6 @@ sepref_def lit_and_ann_of_propagated_st_heur_fast_code
   unfolding fold_tuple_optimizations
   by sepref
 
-declare
-  lit_and_ann_of_propagated_st_heur_fast_code.refine[sepref_fr_rules]
-
-(*TODO Move or kill*)
-definition is_UNSET where [simp]: \<open>is_UNSET x \<longleftrightarrow> x = UNSET\<close>
-lemma tri_bool_is_UNSET_refine_aux:
-  \<open>(\<lambda>x. x = 0, is_UNSET) \<in> tri_bool_rel_aux \<rightarrow> bool_rel \<close>
-  by (auto simp: tri_bool_rel_aux_def)
-
-sepref_definition is_UNSET_impl
-  is \<open>RETURN o (\<lambda>x. x= 0)\<close>
-  :: \<open>(unat_assn' TYPE(8))\<^sup>k \<rightarrow>\<^sub>a bool1_assn\<close>
-  apply (annot_unat_const \<open>TYPE(8)\<close>)
-  by sepref
-
-(*lemmas [sepref_fr_rules] = is_UNSET_impl.refine[FCOMP tri_bool_is_UNSET_refine_aux]*)
-(*END Move*)
-
-(*TODO Move*)
-
-sepref_def is_in_option_lookup_conflict_code
-  is \<open>uncurry (RETURN oo is_in_option_lookup_conflict)\<close>
-  :: \<open>[\<lambda>(L, (c, n, xs)). atm_of L < length xs]\<^sub>a
-        unat_lit_assn\<^sup>k *\<^sub>a conflict_option_rel_assn\<^sup>k \<rightarrow> bool1_assn\<close>
-  unfolding is_in_option_lookup_conflict_alt_def is_in_lookup_conflict_def PROTECT_def
-     is_NOTIN_alt_def[symmetric] conflict_option_rel_assn_def lookup_clause_rel_assn_def
-  by sepref
-
 sepref_def atm_is_in_conflict_st_heur_fast_code
   is \<open>uncurry (atm_is_in_conflict_st_heur)\<close>
   :: \<open>[\<lambda>_. True]\<^sub>a unat_lit_assn\<^sup>k *\<^sub>a isasat_bounded_assn\<^sup>k \<rightarrow> bool1_assn\<close>
@@ -123,17 +46,6 @@ sepref_def atm_is_in_conflict_st_heur_fast_code
    is_NOTIN_def[symmetric] conflict_option_rel_assn_def lookup_clause_rel_assn_def
   unfolding fold_tuple_optimizations atm_in_conflict_lookup_pre_def
   by sepref
-
-declare atm_is_in_conflict_st_heur_fast_code.refine[sepref_fr_rules]
-(*END Move*)
-
-sepref_def (in -) lit_of_last_trail_fast_code
-  is \<open>RETURN o lit_of_last_trail_pol\<close>
-  :: \<open>[\<lambda>(M). fst M \<noteq> []]\<^sub>a trail_pol_fast_assn\<^sup>k \<rightarrow> unat_lit_assn\<close>
-  unfolding lit_of_last_trail_pol_def trail_pol_fast_assn_def
-  by sepref
-
-declare lit_of_last_trail_fast_code.refine[sepref_fr_rules]
 
 lemma tl_state_wl_heurI: \<open>tl_state_wl_heur_pre (a, b) \<Longrightarrow> fst a \<noteq> []\<close>
   \<open>tl_state_wl_heur_pre (a, b) \<Longrightarrow> tl_trailt_tr_pre a\<close>
@@ -153,29 +65,12 @@ lemma tl_state_wl_heur_alt_def:
 sepref_def tl_state_wl_heur_fast_code
   is \<open>tl_state_wl_heur\<close>
   :: \<open>[\<lambda>_. True]\<^sub>a isasat_bounded_assn\<^sup>d \<rightarrow> bool1_assn \<times>\<^sub>a isasat_bounded_assn\<close>
-  supply [[goals_limit=1]] if_splits[split] tl_state_wl_heurI[simp]
+  supply [[goals_limit=1]] if_splits[split] tl_state_wl_heurI[dest]
   unfolding tl_state_wl_heur_alt_def[abs_def] isasat_bounded_assn_def get_trail_wl_heur_def
     vmtf_unset_def bind_ref_tag_def short_circuit_conv
   unfolding fold_tuple_optimizations
   apply (rewrite in \<open>ASSERT \<hole>\<close> fold_tuple_optimizations[symmetric])+
   by sepref
-
-declare
-  tl_state_wl_heur_fast_code.refine[sepref_fr_rules]
-
-definition None_lookup_conflict :: \<open>_ \<Rightarrow> _ \<Rightarrow> conflict_option_rel\<close> where
-\<open>None_lookup_conflict b xs = (b, xs)\<close>
-
-
-sepref_def None_lookup_conflict_impl
-  is \<open>uncurry (RETURN oo None_lookup_conflict)\<close>
-  :: \<open>bool1_assn\<^sup>k *\<^sub>a lookup_clause_rel_assn\<^sup>d \<rightarrow>\<^sub>a conflict_option_rel_assn\<close>
-  unfolding None_lookup_conflict_def conflict_option_rel_assn_def
-    lookup_clause_rel_assn_def
-  by sepref
-
-sepref_register None_lookup_conflict
-declare None_lookup_conflict_impl.refine[sepref_fr_rules]
 
 
 definition extract_values_of_lookup_conflict :: \<open>conflict_option_rel \<Rightarrow> bool\<close> where
