Weidenbach_Book/IsaSAT/IsaSAT_Trail_LLVM.thy
@@ -3,40 +3,6 @@ imports IsaSAT_Literals_LLVM IsaSAT_Trail
 begin
 
 
-type_synonym tri_bool_assn = \<open>8 word\<close>
-
-definition \<open>tri_bool_rel_aux \<equiv> { (0::nat,None), (2,Some True), (3,Some False) }\<close>
-definition \<open>tri_bool_rel \<equiv> unat_rel' TYPE(8) O tri_bool_rel_aux\<close>
-abbreviation \<open>tri_bool_assn \<equiv> pure tri_bool_rel\<close>
-lemmas [fcomp_norm_unfold] = tri_bool_rel_def[symmetric]
-
-lemma tri_bool_UNSET_refine_aux: \<open>(0,UNSET)\<in>tri_bool_rel_aux\<close>
-  and tri_bool_SET_TRUE_refine_aux: \<open>(2,SET_TRUE)\<in>tri_bool_rel_aux\<close>
-  and tri_bool_SET_FALSE_refine_aux: \<open>(3,SET_FALSE)\<in>tri_bool_rel_aux\<close>
-  and tri_bool_eq_refine_aux: \<open>((=),tri_bool_eq) \<in> tri_bool_rel_aux\<rightarrow>tri_bool_rel_aux\<rightarrow>bool_rel\<close>
-  by (auto simp: tri_bool_rel_aux_def tri_bool_eq_def)
-
-sepref_def tri_bool_UNSET_impl is [] \<open>uncurry0 (RETURN 0)\<close> :: \<open>unit_assn\<^sup>k \<rightarrow>\<^sub>a unat_assn' TYPE(8)\<close>
-  apply (annot_unat_const \<open>TYPE(8)\<close>)
-  by sepref
-
-sepref_def tri_bool_SET_TRUE_impl is [] \<open>uncurry0 (RETURN 2)\<close> :: \<open>unit_assn\<^sup>k \<rightarrow>\<^sub>a unat_assn' TYPE(8)\<close>
-  apply (annot_unat_const \<open>TYPE(8)\<close>)
-  by sepref
-
-sepref_def tri_bool_SET_FALSE_impl is [] \<open>uncurry0 (RETURN 3)\<close> :: \<open>unit_assn\<^sup>k \<rightarrow>\<^sub>a unat_assn' TYPE(8)\<close>
-  apply (annot_unat_const \<open>TYPE(8)\<close>)
-  by sepref
-
-sepref_def tri_bool_eq_impl [llvm_inline] is [] \<open>uncurry (RETURN oo (=))\<close> :: \<open>(unat_assn' TYPE(8))\<^sup>k *\<^sub>a (unat_assn' TYPE(8))\<^sup>k \<rightarrow>\<^sub>a bool1_assn\<close>
-  by sepref
-
-lemmas [sepref_fr_rules] =
-  tri_bool_UNSET_impl.refine[FCOMP tri_bool_UNSET_refine_aux]
-  tri_bool_SET_TRUE_impl.refine[FCOMP tri_bool_SET_TRUE_refine_aux]
-  tri_bool_SET_FALSE_impl.refine[FCOMP tri_bool_SET_FALSE_refine_aux]
-  tri_bool_eq_impl.refine[FCOMP tri_bool_eq_refine_aux]
-
 type_synonym trail_pol_fast_assn =
    \<open>32 word array_list64 \<times> tri_bool_assn larray64 \<times> 32 word larray64 \<times>
      64 word larray64 \<times> 32 word \<times>
@@ -94,6 +60,13 @@ sepref_def polarity_pol_fast_code
   unfolding polarity_pol_def option.case_eq_if polarity_pol_pre_def
     trail_pol_fast_assn_def
   supply [[goals_limit = 1]]
+  by sepref
+
+sepref_def polarity_pol_fast
+  is \<open>uncurry (mop_polarity_pol)\<close>
+  :: \<open>trail_pol_fast_assn\<^sup>k *\<^sub>a unat_lit_assn\<^sup>k \<rightarrow>\<^sub>a tri_bool_assn\<close>
+  unfolding mop_polarity_pol_def trail_pol_fast_assn_def
+    polarity_pol_def polarity_pol_pre_def
   by sepref
 
 
@@ -283,14 +256,6 @@ schematic_goal mk_free_trail_pol_fast_assn[sepref_frame_free_rules]: \<open>MK_F
   unfolding trail_pol_fast_assn_def
   by synthesize_free
 
-(*TODO Move*)
-
-sepref_def polarity_pol_fast
-  is \<open>uncurry (mop_polarity_pol)\<close>
-  :: \<open>trail_pol_fast_assn\<^sup>k *\<^sub>a unat_lit_assn\<^sup>k \<rightarrow>\<^sub>a tri_bool_assn\<close>
-  unfolding mop_polarity_pol_def trail_pol_fast_assn_def
-    polarity_pol_def polarity_pol_pre_def
-  by sepref
 
 experiment begin
 
